More primitives from the `Atomic` module.

osiris/src/Rocqify.ml
@@ -356,8 +356,14 @@ let rec expr (e : expr) =
   | EStore (e1, e2) ->
       c "EStore" [ expr e1; expr e2 ]
 
+  | EExchange (e1, e2) ->
+      c "EExchange" [ expr e1; expr e2 ]
+
   | ECAS (e1, e2, e3) ->
       c "ECAS" [ expr e1; expr e2; expr e3 ]
+
+  | EIgnore e ->
+      c "EIgnore" [ expr e ]
 
   | EFork (e1, e2) ->
       c "EFork" [ expr e1; expr e2 ]
