rocq-osiris/interp/E2O.ml
@@ -141,7 +141,9 @@ let rec expr : E.expr -> O.expr = function
   | ERef e -> ERef (expr e)
   | ELoad e -> ELoad (expr e)
   | EStore (e1, e2) -> EStore (expr e1, expr e2)
+  | EExchange (e1, e2) -> EExchange (expr e1, expr e2)
   | ECAS (e1, e2, e3) -> ECAS (expr e1, expr e2, expr e3)
+  | EIgnore e -> EIgnore (expr e)
   | EFork (e1, e2) -> EFork (expr e1, expr e2)
   | EJoin e -> EJoin (expr e)
 
